feat: Handshake-to-HW `fork` circuit (#1925)
We add the encoding of an `fork` circuit lowered with CIRCT from the
handshake to the RTL level.

---------

Co-authored-by: Yann Herklotz <git@yannherklotz.com>

SSA/Projects/CIRCT/HandshakeToHW/add.lean
@@ -2,94 +2,194 @@ import SSA.Projects.CIRCT.Stream.Basic
 import SSA.Projects.CIRCT.Stream.Lemmas
 import SSA.Projects.CIRCT.Register.Basic
 import SSA.Projects.CIRCT.Register.Lemmas
-
+import SSA.Projects.CIRCT.Handshake.Handshake
 namespace HandshakeStream
 
-/-
-Handshake program (https://github.com/opencompl/DC-semantics-simulation-evaluation/blob/main/benchmarks/add_naive/handshake.mlir) :
+/-!
+  # Add
 
-handshake.func @add(%a : i32, %b : i32) -> i32{
-    %add1 = comb.add %a, %a : i32
-    %add2 = comb.add %add1, %b : i32
-    return %add2: i32
-}
-
-Lowered program (https://github.com/opencompl/DC-semantics-simulation-evaluation/blob/main/benchmarks/add_naive/hw-esi-hw.mlir):
-
-module {
-  hw.module @add(in %a : i32, in %a_valid : i1, in %b : i32, in %b_valid : i1, in %clk : !seq.clock, in %rst : i1, in %out0_ready : i1, out a_ready : i1, out b_ready : i1, out out0 : i32, out out0_valid : i1) {
-    %false = hw.constant false
-    %c0_i0 = hw.constant 0 : i0
-    %c0_i0_0 = hw.constant 0 : i0
-    %c0_i0_1 = hw.constant 0 : i0
-    %false_2 = hw.constant false
-    %true = hw.constant true
-    %0 = comb.xor %12, %true : i1
-    %1 = comb.and %5, %0 : i1
-    %emitted_0 = seq.compreg sym @emitted_0 %1, %clk reset %rst, %false_2 : i1
-    %2 = comb.xor %emitted_0, %true : i1
-    %3 = comb.and %2, %a_valid : i1
-    %4 = comb.and %16, %3 : i1
-    %5 = comb.or %4, %emitted_0 {sv.namehint = "done0"} : i1
-    %6 = comb.xor %12, %true : i1
-    %7 = comb.and %11, %6 : i1
-    %emitted_1 = seq.compreg sym @emitted_1 %7, %clk reset %rst, %false_2 : i1
-    %8 = comb.xor %emitted_1, %true : i1
-    %9 = comb.and %8, %a_valid : i1
-    %10 = comb.and %16, %9 : i1
-    %11 = comb.or %10, %emitted_1 {sv.namehint = "done1"} : i1
-    %12 = comb.and %5, %11 {sv.namehint = "allDone"} : i1
-    %13 = comb.extract %a from 0 : (i32) -> i31
-    %14 = comb.concat %13, %false : i31, i1
-    %c0_i0_3 = hw.constant 0 : i0
-    %c0_i0_4 = hw.constant 0 : i0
-    %15 = comb.and %b_valid, %9, %3 : i1
-    %16 = comb.and %out0_ready, %15 : i1
-    %17 = comb.add %14, %b : i32
-    hw.output %12, %16, %17, %15 : i1, i1, i32, i1
-  }
-}
--/
-
-
-
-/--
-  `add` performs two additions given inputs `a` and `b`: (a + a) + b
+  We add a circuit that given two inputs `a` and `b` performs two additions: `(a + a) + b`.
 
   The hardware (lowered) module is a function over the `Stream'` type,
   which does not contain `Option` values, because at this level
   of abstractions the content of streams has been concretized.
+  We ignore buffers.
+
+  See: https://github.com/opencompl/DC-semantics-simulation-evaluation/commit/bf86f7247a767d97516a05a29e313634e5172398
+
 -/
-def add
-  (xst : Stream' (wiresStruc 2 3)) :
-    Stream' (wiresStruc 1 3) :=
+
+/--
+  Handshake program after buffers' insertion and materialization:
+
+  module {
+    handshake.func @add(%arg0: index, %arg1: index, %arg2: none, ...) -> (index, none) attributes {argNames = ["arg0", "arg1", "arg2"], resNames = ["out0", "out1"]} {
+      %0:2 = fork [2] %arg0 : index
+      %1 = buffer [2] seq %arg2 : none
+      %2 = arith.addi %0#0, %0#1 : index
+      %3 = buffer [2] seq %2 : index
+      %4 = arith.addi %3, %arg1 : index
+      %5 = buffer [2] seq %4 : index
+      return %5, %1 : index, none
+    }
+  }
+
+  We define it based on a synchroniing wrapper, that first synchronizes the input streams and
+  then applies the operation.
+
+  We ignore the semantics of buffers.
+-/
+def add_handshake (a b : Stream' (Option (BitVec 64))) :=
+  let ⟨fork_0, fork_1⟩ := HandshakeOp.fork a
+  let addi_1 := syncMap₂ BitVec.add fork_0 fork_1
+  let addi_2 := syncMap₂ BitVec.add addi_1 b
+  addi_2
+
+/--
+  First RTL module:
+
+  hw.module @handshake_fork_in_ui64_out_ui64_ui64(in %in0 : i64, in %in0_valid : i1, in %clock : !seq.clock, in %reset : i1, in %out0_ready : i1, in %out1_ready : i1, out in0_ready : i1, out out0 : i64, out out0_valid : i1, out out1 : i64, out out1_valid : i1) {
+    %true = hw.constant true
+    %false = hw.constant false
+    %0 = comb.xor %12, %true : i1
+    %1 = comb.and %5, %0 : i1
+    %emitted_0 = seq.compreg sym @emitted_0 %1, %clock reset %reset, %false : i1
+    %2 = comb.xor %emitted_0, %true : i1
+    %3 = comb.and %2, %in0_valid : i1
+    %4 = comb.and %out0_ready, %3 : i1
+    %5 = comb.or %4, %emitted_0 {sv.namehint = "done0"} : i1
+    %6 = comb.xor %12, %true : i1
+    %7 = comb.and %11, %6 : i1
+    %emitted_1 = seq.compreg sym @emitted_1 %7, %clock reset %reset, %false : i1
+    %8 = comb.xor %emitted_1, %true : i1
+    %9 = comb.and %8, %in0_valid : i1
+    %10 = comb.and %out1_ready, %9 : i1
+    %11 = comb.or %10, %emitted_1 {sv.namehint = "done1"} : i1
+    %12 = comb.and %5, %11 {sv.namehint = "allDone"} : i1
+    hw.output %12, %in0, %3, %in0, %9 : i1, i64, i1, i64, i1
+  }
+-/
+def handshake_fork_in_ui64_out_ui64_ui64
+    (instruc : Stream' (wiresStruc 1 3 64)) :
+    Stream' (wiresStruc 2 3 64)  :=
+  register_wrapper_generalized
+    (inputs := instruc)
+    (init_regs := {result := #v[], signals := #v[0#1, 0#1]})
+    (outops := 2)
+    (outsigs := 3)
+    (update_fun :=
+      fun (inp, regs) =>
+        let v2 := regs.signals[0] ^^^ 1#1 -- emitted_0
+        let v3 := v2 &&& inp.signals[0] -- in0_valid
+        let v4 := inp.signals[1] &&& v3 -- out0_ready
+        let v5 := v4 ||| regs.signals[0]
+        let v8 := regs.signals[1] ^^^ 1#1 -- emitted_1
+        let v9 := v8 &&& inp.signals[0] -- in0_valid
+        let v10 := inp.signals[2] &&& v9 -- out1_ready
+        let v11 := v10 ||| regs.signals[1]
+        let v12 := v5 &&& v11
+        let v0 := v12 ^^^ 1#1
+        let v1 := v5 &&& v0
+        let v6 := v12 ^^^ 1#1
+        let v7 := v11 &&& v6
+        let updated_reg0 := v1
+        let updated_reg1 := v7
+        ⟨{result := #v[inp.result[0], inp.result[0]], signals := #v[v12, v3, v9]},
+                            {result := #v[], signals := #v[updated_reg0, updated_reg1]}⟩
+        )
+
+/--
+  Second RTL module:
+
+  hw.module @arith_addi_in_ui64_ui64_out_ui64(in %in0 : i64, in %in0_valid : i1, in %in1 : i64, in %in1_valid : i1, in %out0_ready : i1, out in0_ready : i1, out in1_ready : i1, out out0 : i64, out out0_valid : i1) {
+    %0 = comb.and %in0_valid, %in1_valid : i1
+    %1 = comb.and %out0_ready, %0 : i1
+    %2 = comb.add %in0, %in1 : i64
+    hw.output %1, %1, %2, %0 : i1, i1, i64, i1
+  }
+
+-/
+def arith_addi_in_ui64_ui64_out_ui64
+  (xst : Stream' (wiresStruc 2 3 64)) :
+    Stream' (wiresStruc 1 3 64) :=
   register_wrapper_generalized
               (inputs := xst)
-              (init_regs := {result := #v[], signals := #v[0#1, 0#1]})
+              (init_regs := {result := #v[], signals := #v[]})
               (outops := 1)
               (outsigs := 3)
               (update_fun :=
                         fun (inp, regs) =>
-                            let v2 := BitVec.xor regs.signals[0] 1#1
-                            let v8 := BitVec.xor regs.signals[1] 1#1
-                            let v3 := BitVec.and v2 inp.signals[0] -- inp a_valid
-                            let v9 := BitVec.and v8 inp.signals[0] -- inp a_valid
-                            let v15 := BitVec.and inp.signals[1] (BitVec.and v9 v3) -- inp b_valid
-                            let v16 := BitVec.and inp.signals[2] v15 --inp out_ready
-                            let v10 := BitVec.and v16 v9
-                            let v4 := BitVec.and v16 v3
-                            let v11 := BitVec.or v10 regs.signals[1] -- emitted_1
-                            let v5 := BitVec.or v4 regs.signals[0] -- emitted_0
-                            let v12 := BitVec.and v5 v11
-                            let v0 := BitVec.xor v12 1#1
-                            let v1 := BitVec.and v5 v0
-                            let v6 := BitVec.xor v12 1#1
-                            let v7 := BitVec.and v11 v6
-                            let v13 := BitVec.extractLsb' 0 31 inp.result[0] -- a
-                            let v14 := BitVec.concat v13 false
-                            let v17 : BitVec 32 := BitVec.add v14 inp.result[1] -- b
-                            let updated_reg0 := v1
-                            let updated_reg1 := v7
-                           ⟨{result := #v[v17], signals := #v[v12, v16, v15]},
-                            {result := #v[], signals := #v[updated_reg0, updated_reg1]}⟩
+                            let v0 := inp.signals[0] &&& inp.signals[1] -- in0_valid &&& in1_valid
+                            let v1 := inp.signals[2] &&& v0 -- out0_ready
+                            let v2 := inp.result[0] + inp.result[1]
+                           ⟨{result := #v[v2], signals := #v[v1, v1, v0]},
+                            {result := #v[], signals := #v[]}⟩
                 )
+
+/--
+  Third RTL module:
+
+    hw.module @add(in %arg0 : i64, in %arg0_valid : i1, in %arg1 : i64, in %arg1_valid : i1, in %arg2 : i0, in %arg2_valid : i1, in %clock : !seq.clock, in %reset : i1, in %out0_ready : i1, in %out1_ready : i1, out arg0_ready : i1, out arg1_ready : i1, out arg2_ready : i1, out out0 : i64, out out0_valid : i1, out out1 : i0, out out1_valid : i1) {
+
+      %handshake_fork0.in0_ready, %handshake_fork0.out0, %handshake_fork0.out0_valid, %handshake_fork0.out1, %handshake_fork0.out1_valid =
+          hw.instance "handshake_fork0" @handshake_fork_in_ui64_out_ui64_ui64
+              (in0: %arg0: i64, in0_valid: %arg0_valid: i1, clock: %clock: !seq.clock, reset: %reset: i1, out0_ready: %arith_addi0.in0_ready: i1, out1_ready: %arith_addi0.in1_ready: i1) ->
+              (in0_ready: i1, out0: i64, out0_valid: i1, out1: i64, out1_valid: i1)
+
+      %arith_addi0.in0_ready, %arith_addi0.in1_ready, %arith_addi0.out0, %arith_addi0.out0_valid =
+          hw.instance "arith_addi0" @arith_addi_in_ui64_ui64_out_ui64
+            (in0: %handshake_fork0.out0: i64, in0_valid: %handshake_fork0.out0_valid: i1, in1: %handshake_fork0.out1: i64, in1_valid: %handshake_fork0.out1_valid: i1, out0_ready: %arith_addi1.in0_ready: i1) ->
+            (in0_ready: i1, in1_ready: i1, out0: i64, out0_valid: i1)
+
+      %arith_addi1.in0_ready, %arith_addi1.in1_ready, %arith_addi1.out0, %arith_addi1.out0_valid =
+          hw.instance "arith_addi1" @arith_addi_in_ui64_ui64_out_ui64
+            (in0: %arith_addi0.out0: i64, in0_valid: %arith_addi0.out0_valid: i1, in1: %arg1: i64, in1_valid: %arg1_valid: i1, out0_ready: %out0_ready: i1) ->
+            (in0_ready: i1, in1_ready: i1, out0: i64, out0_valid: i1)
+
+      hw.output %handshake_fork0.in0_ready, %arith_addi1.in1_ready, %out1_ready, %arith_addi1.out0, %arith_addi1.out0_valid, %arg2, %arg2_valid : i1, i1, i1, i64, i1, i0, i1
+    }
+-/
+-- def add_rtl
+  /-
+    xst.result[0] = arg0
+    xst.result[1] = arg1
+    xst.signals[0] = arg0_valid
+    xst.signals[1] = arg1_valid
+    xst.signals[2] = arg2
+    xst.signals[3] = arg2_valid
+    xst.signals[4] = out0_ready
+    xst.signals[5] = out1_ready
+  -/
+  -- (inp : Stream' (wiresStruc 2 6 64)) : Stream' (wiresStruc 1 6 64) :=
+    -- let arg0 := inp.resul[0]
+    -- let arg1 := inp.resut[1]
+    -- let arg0_valid := inp.signal[0]
+    -- let arg1_valid := inp.signal[1]
+    -- let arg2 := inp.signal[2]
+    -- let arg2_valid := inp.signal[3]
+    -- let out0_ready := inp.signal[4]
+    -- let out1_ready := inp.signal[5]
+    -- let fork_in : wiresStruc 1 3 64 :=
+    --         {result := #v[arg0],
+    --           /- `out0_ready` and `out1_ready` are incorrect (see above).
+    --             we need to iteratively compute all the values in the current state of the circuit
+    --             (until fixed point). -/
+    --           signals := #v[arg0_valid, out0_ready, out1_ready]}
+    -- sorry
+
+
+theorem lowering_correctness
+  (a b : Stream (BitVec 64)) -- handshake level
+  (a_readyvalid b_readyvalid : wiresStructStream 1 2 64) -- rtl level
+  (sig_readyValid : Vector (Stream' (BitVec 1)) 3) -- extra input signal
+  (hsig : ReadyValid sig_readyValid sig)
+  (hsig_a : ReadyValidStruc a_readyvalid a) (hsig_b : ReadyValidStruc b_readyvalid b) :
+    let inp : wiresStructStream 2 6 64 := {
+      result := #v[a_readyvalid.result[0], b_readyvalid.result[0]]
+      signals := #v[a_readyvalid.signals[1], b_readyvalid.signals[1],
+                    sig_readyValid[0], sig_readyValid[2],
+                    a_readyvalid.signals[0], b_readyvalid.signals[0]]}
+    let inp' := streams_to_wires inp
+    let rtl' := add_rtl inp'
+    let rtl := wires_to_streams rtl'
+    (add_handshake a b) ~ rtl.result[0] := by sorry
