SSA/Projects/CIRCT/HandshakeToHW/file.lean
@@ -1,0 +1,15 @@
+
+
+inductive HVectorNormal : List (Type u) -> (Type (u + 1))
+| nil : HVectorNormal []
+| cons (t : Type u) (x : t) (rest : HVectorNormal ts) : HVectorNormal (t :: ts)
+
+#check HVectorNormal
+def foo : HVectorNormal [String, Int] := .cons String "foo" <| .cons Int 42 <| .nil
+
+-- mlitty : Type
+-- mlirty.denote : mlirty -> Type
+
+inductive HVectorLeanMLIR (denote : mlirty → Type u) : List mlirty → Type u
+| nil : HVectorLeanMLIR denote []
+| cons (t : mlirty) (x : denote t) (rest : HVectorLeanMLIR denote ts) : HVectorLeanMLIR denote (t :: ts)
