SSA/Projects/CIRCT/HandshakeToHW/simple_example.lean
@@ -1,0 +1,174 @@
+import SSA.Projects.CIRCT.Register.Basic
+import SSA.Projects.CIRCT.Stream.Basic
+
+open HandshakeStream
+
+def streams_to_vec' {α : Type u} {n : Nat} (xv : Vector (Stream' α) n) : Stream' (Vector α n) :=
+  /- `map` applies `fun (s : Stream' α) => s i` to every element in `xv` -/
+  fun (i : Nat) => xv.map (fun (s : Stream' α) => s i)
+
+-- /--
+--   Map the `i`-th element of stream `s` in `xv` to the output heterogeneous vector, using `Stream'`.
+-- -/
+-- def streams'_to_hvec {α : Type u} {n : Nat} (xv : HVector f lin) : Stream' (HVector f lin) :=
+--   /- `map` applies `fun (s : Stream' α) => s i` to every element in `xv` -/
+--   fun (f, lin) => xv.map (fun (s : Stream' α) => s i)
+
+/--
+  Map each element at the `k`-th position of `xv` to the `k`-th stream of the output, using `Stream'`.
+-/
+def vec_to_streams' {α : Type u} {n : Nat} (xv : Stream' (Vector α n)) : Vector (Stream' α) n :=
+  /- `.ofFn` creates a vector with `n` elements (for each `k` from `0` to `n - 1`),
+      where each element is a stream `fun (i : Nat) => ...` containing the `k`-th element of the
+      `i`-th element of stream `xv`.
+  -/
+  Vector.ofFn (fun (k : Fin n) => fun (i : Nat) => (xv i).get k)
+
+abbrev opt_bitvec (n : Nat) : Type := Option (BitVec n)
+
+abbrev stream_opt_bitvec (n : Nat) : Type := Stream' (opt_bitvec n)
+
+def convertVecToStream {l : List Nat} (xv : HVector stream_opt_bitvec l) : Stream' (HVector opt_bitvec l) :=
+  fun (i : Nat) =>
+    xv.map (fun {n : Nat} (s : stream_opt_bitvec n) => s i)
+
+def convertStreamToVec {l : List Nat} (xv : Stream' (HVector opt_bitvec l)) : HVector stream_opt_bitvec l :=
+  HVector.ofFn stream_opt_bitvec l (fun (k : Fin l.length) => fun (i : Nat) => (xv i).get k)
+
+/--
+  A module with a register that keeps the stores the "ready" value and outputs a couple where:
+  · the first element is true if the value of the register and the current input are true
+  · the second element is true
+-/
+def output_const (input : HVector stream_opt_bitvec [1]) : HVector stream_opt_bitvec [1, 1] :=
+  let hv := het_register_wrapper
+              (ls := [1]) (lout := [1, 1])
+              (inputs := convertVecToStream input)
+              (init_regs := HVector.cons (some true) HVector.nil)
+              (update_fun :=
+                fun (inp, regs) =>
+                  let e := (regs.get ⟨0, by simp⟩)
+                  let i := (inp.get ⟨0, by simp⟩)
+                  let updatedreg : HVector opt_bitvec [1] := HVector.cons (inp.get ⟨0, by simp⟩) (HVector.nil)
+                  match e, i with
+                  | some e', some i' =>
+                      let e'' := e'[0]
+                      let i'' := i'[0]
+                      let b := e''.and i''
+                      let output : HVector opt_bitvec [1, 1] := HVector.cons (some b) (HVector.cons (some true) HVector.nil)
+                      ⟨updatedreg, output⟩
+                  | _, _ =>
+                    let output : HVector opt_bitvec [1, 1] := HVector.cons (some false) (HVector.cons (some true) HVector.nil)
+                    ⟨updatedreg, output⟩)
+  convertStreamToVec hv
+
+
+/--
+  A module with a register that flips between [true, false].
+  The "ready" output should reflect the state of the register.
+  It doesn't have to do anything with the inputs.
+-/
+def sink (input : HVector stream_opt_bitvec [1, 1]) : HVector stream_opt_bitvec [1] :=
+    let values := [true, true, false]
+    let hv := het_register_wrapper
+              (ls := [1]) (lout := [1])
+              (inputs := convertVecToStream input)
+              (init_regs := HVector.cons (some true) HVector.nil)
+              (update_fun :=
+                fun (inp, regs) =>
+                  let e := (regs.get ⟨0, by simp⟩)
+                  match e with
+                  | some e' =>
+                    if e'[0] = true then
+                      /- TODO: Luisa could not find a way to make it flip [true, true, false] -/
+                      let output : HVector opt_bitvec [1] := HVector.cons (some true) HVector.nil
+                      let updatedreg : HVector opt_bitvec [1] := HVector.cons (some false) HVector.nil
+                      ⟨updatedreg, output⟩
+                    else
+                      let output : HVector opt_bitvec [1] := HVector.cons (some false) HVector.nil
+                      let updatedreg : HVector opt_bitvec [1] := HVector.cons (some true) HVector.nil
+                      ⟨updatedreg, output⟩
+                  | none =>
+                    let output : HVector opt_bitvec [1] := HVector.cons none HVector.nil
+                    let updatedreg : HVector opt_bitvec [1] := HVector.cons none HVector.nil
+                    ⟨updatedreg, output⟩)
+    convertStreamToVec hv
+
+def bufferConst (input : HVector stream_opt_bitvec [1]) : HVector stream_opt_bitvec [32, 1] :=
+    let hv := het_register_wrapper
+              (inputs := convertVecToStream input)
+              (init_regs := HVector.cons (.some 0#32) HVector.nil)
+              (update_fun :=
+                fun (inp, regs) =>
+                  let inVal := inp.get ⟨0, by simp⟩
+                  let regVal : BitVec 32 := regs.get ⟨0, by simp⟩ |>.get!
+                  if inVal == .some 1#1
+                  then 
+                    let updatedReg := HVector.cons (.some (regVal + 1#32)) .nil
+                    (updatedReg, HVector.cons (.some regVal) <| .cons 1#1 .nil)
+                  else
+                    (regs, HVector.cons (.some regVal) <| .cons 1#1 .nil))
+    convertStreamToVec hv
+
+def elastic_fifo_inner (input : HVector stream_opt_bitvec [32, 1, 1]) : HVector stream_opt_bitvec [32, 1, 1] :=
+    let hv : Stream' (Option (HVector opt_bitvec [32, 1, 1])) := het_register_wrapper'
+              (inputs := convertVecToStream input)
+              -- Memory, Full, Empty
+              (init_regs := HVector.cons 0#32 <| .cons 0#1 <| .cons 1#1 HVector.nil)
+              (update_fun :=
+                fun (inp, regs) => Id.run <| do
+                  let defval : HVector opt_bitvec [32, 1, 1] := HVector.cons .none <| .cons .none <| .cons .none .nil
+                  let .some ins := inp.get ⟨0, by simp⟩
+                    | .none
+                  let .some ins_valid := inp.get ⟨1, by simp⟩
+                    | .none
+                  let .some outs_ready := inp.get ⟨2, by simp⟩
+                    | .none
+                  let Memory := regs.get ⟨0, by simp⟩ |>.get!
+                  let Full := regs.get ⟨1, by simp⟩ |>.get!
+                  let Empty := regs.get ⟨2, by simp⟩ |>.get!
+                  let ins_ready := BitVec.or (BitVec.not Full) outs_ready
+                  let ReadEn := BitVec.and outs_ready (BitVec.not Empty)
+                  let outs_valid := BitVec.not Empty
+                  let WriteEn := BitVec.and ins_valid (BitVec.or (BitVec.not Full) outs_ready)
+                  let outs := Memory
+                  let mut newMemory := Memory
+                  sorry)
+    sorry
+
+def het_fix_wrapper (fuel : Nat) (s : Stream' (HVector opt_bitvec l)) (f : Stream' (HVector opt_bitvec l) → Stream' (HVector opt_bitvec l)) :
+    Stream' (HVector opt_bitvec l) :=
+  match fuel with
+  | 0 => s
+  | n+1 => het_fix_wrapper n (f s) f
+
+def het_fix_wrapper_single (fuel : Nat) (s : HVector opt_bitvec l) (f : HVector opt_bitvec l → HVector opt_bitvec l) : (HVector opt_bitvec l) :=
+  match fuel with
+  | 0 => s
+  | n+1 => het_fix_wrapper_single n (f s) f
+
+def compute_module' (input : Stream' (HVector opt_bitvec [1])) : Stream' (HVector opt_bitvec [1]) :=
+  let inputStream := convertStreamToVec input
+  let const_outs := output_const inputStream
+  convertVecToStream <| sink const_outs
+
+/- def compute_module_single' (input : Stream' (HVector opt_type [1])) : Stream' (HVector opt_type [1]) :=
+  let inputStream := convertStreamToVec input
+  let const_outs := output_const inputStream
+  let sink_outs := sink const_outs
+  convertVecToStream <| (Stream'.map (het_fix_wrapper_single 100 (f := ??)) sink_outs) -/
+
+def complete_module :=
+  het_fix_wrapper 2 (fun _ => .cons .none <| .nil) compute_module'
+
+instance : ToString (Stream' (HVector opt_bitvec [1])) where
+  toString s :=
+    Id.run do
+      let mut result := ""
+      for i in [0:10] do
+        let elm := s i
+        let elm' := elm.get ⟨0, sorry⟩
+        result := result ++ toString elm' ++ "\n"
+      return result
+
+#eval! timeit "" <| IO.println <| complete_module
